fairness/lawyer/obligations_am.v
@@ -1,0 +1,38 @@
+From stdpp Require Import namespaces. 
+From iris.proofmode Require Import tactics.
+From trillium.fairness Require Import utils.
+From trillium.fairness.lawyer Require Import obligations_model action_model.
+
+
+Section ObligationsAM.
+  Context `(OP: ObligationsParams Degree Level Locale LIM_STEPS).
+  Context `{Countable Locale}.
+  Context `{Inhabited Locale}.
+  Let OM := ObligationsModel OP.
+
+  Definition obls_ns: namespace := nroot .@ "obligations".
+  Definition obls_act: Action := coPpick (↑ obls_ns).
+
+  Inductive obls_AM_trans: ProgressState OP → Action * option Locale → ProgressState OP → Prop :=
+  | oam_step δ1 ρ δ2
+      (STEP: om_trans OP δ1 ρ δ2):
+  obls_AM_trans δ1 (obls_act, Some ρ) δ2. 
+  
+  Global Instance OM_st_eqdec: EqDecision (ProgressState OP).
+  Proof. solve_decision. Qed. 
+
+  Global Instance OM_st_inh: Inhabited (ProgressState OP).
+  Proof.
+    constructor. exact {|
+      ps_cps := ∅;
+      ps_sigs := ∅;
+      ps_obls := ∅;
+      ps_eps := ∅;
+      ps_phases := ∅;
+      ps_exc_bound := 0;
+  |}.
+  Qed. 
+    
+  Definition ObligationsAM: ActionModel := {| amTrans := obls_AM_trans |}.
+
+End ObligationsAM.
